theories/adequacy.v
@@ -1,6 +1,6 @@
 From iris.proofmode Require Import tactics.
 From iris.program_logic Require Export adequacy weakestpre.
-From iris.algebra Require Import csum excl auth cmra_big_op gmap.
+From iris.algebra Require Import csum excl auth cmra_big_op gmap frac_agree.
 From iris.base_logic.lib Require Import ghost_map ghost_var.
 From isla Require Export ghost_state lifting.
 Set Default Proof Using "Type".
@@ -12,7 +12,7 @@ Class islaPreG Σ := PreIslaG {
   heap_pre_struct_regs_inG :> ghost_mapG Σ (string * string) valu;
   heap_pre_mem_inG :> ghost_mapG Σ addr byte;
   heap_pre_backed_mem_inG :> inG Σ (backed_memUR);
-  heap_pre_spec_inG :> ghost_varG Σ (list seq_label);
+  heap_pre_spec_inG :> inG Σ (frac_agreeR $ (list seq_label -d> PropO));
 }.
 
 Definition islaΣ : gFunctors :=
@@ -21,7 +21,7 @@ Definition islaΣ : gFunctors :=
    ghost_mapΣ (string * string) valu;
    ghost_mapΣ addr byte;
    GFunctor (constRF backed_memUR);
-   ghost_varΣ (list seq_label)].
+   GFunctor (frac_agreeR $ (list seq_label -d> PropO))].
 
 Instance subG_islaPreG {Σ} : subG islaΣ Σ → islaPreG Σ.
 Proof. solve_inG. Qed.
@@ -32,30 +32,31 @@ Definition initial_local_state (regs : reg_map) : seq_local_state := {|
   seq_nb_state := false;
 |}.
 
-Lemma isla_adequacy Σ `{!islaPreG Σ} (instrs : gmap addr (list trc)) (mem : mem_map) (regs : list reg_map) κsspec t2 σ2 κs n:
+Lemma isla_adequacy Σ `{!islaPreG Σ} (instrs : gmap addr (list trc)) (mem : mem_map) (regs : list reg_map) (Pκs : _ → Prop) t2 σ2 κs n:
+  Pκs [] →
   (∀ {HG : islaG Σ},
-    ⊢ instr_table instrs -∗ backed_mem (dom _ mem) -∗ spec_trace κsspec
+    ⊢ instr_table instrs -∗ backed_mem (dom _ mem) -∗ spec_trace Pκs
     ={⊤}=∗ [∗ list] rs ∈ regs, ∀ (_ : threadG), ([∗ map] r↦v∈rs, r ↦ᵣ v) -∗ WPasm []) →
   nsteps n (initial_local_state <$> regs, {| seq_instrs := instrs; seq_mem := mem |}) κs (t2, σ2) →
-  (∀ e2, e2 ∈ t2 → not_stuck e2 σ2) ∧
-  κs `prefix_of` κsspec.
+  (∀ e2, e2 ∈ t2 → not_stuck e2 σ2) ∧ Pκs κs.
 Proof.
-  move => Hwp.
+  move => ? Hwp.
   apply: wp_strong_adequacy => ?.
   set i := to_instrtbl instrs.
   set bm := to_backed_mem (dom _ mem).
   iMod (own_alloc (i)) as (γi) "#Hi" => //.
   iMod (own_alloc (bm)) as (γbm) "#Hb" => //.
-  iMod (ghost_var_alloc κsspec) as (γs) "[Hs1 Hs2]".
+  iMod (own_alloc (to_frac_agree (A:= _ -d> _) (1/2 + 1/2) Pκs)) as (γs) "Hs" => //.
+  rewrite frac_agree_op. iDestruct "Hs" as "[Hs1 Hs2]".
   iMod (ghost_map_alloc mem) as (γm) "[Hm1 Hm2]".
 
-  set (HheapG := HeapG _ _ γi _ _ _ γm _ γbm κs κsspec _ γs).
+  set (HheapG := HeapG _ _ γi _ _ _ γm _ γbm κs Pκs _ γs).
   set (HislaG := IslaG _ _ HheapG).
   iAssert (instr_table instrs) as "#His". { by rewrite instr_table_eq. }
   iAssert (backed_mem (dom _ mem)) as "#Hbm". { by rewrite backed_mem_eq. }
 
   iMod (Hwp HislaG with "His Hbm [Hs1]") as "Hwp". {
-    rewrite spec_trace_eq. iFrame.
+    rewrite spec_trace_eq. iExists _. rewrite spec_trace_raw_eq. by iFrame.
   }
 
   iModIntro.
@@ -76,10 +77,10 @@ Proof.
       * move => ?? [?[??]]. simplify_map_eq.
   - iIntros (?????) "(Hspec&?) ? ?".
     iApply fupd_mask_intro; [done|]. iIntros "_".
-    iDestruct "Hspec" as (? ? Hκs Hspec) "?".
+    iDestruct "Hspec" as (Pκs' ? Hκs Hspec ?) "?".
     simpl in *. subst.
     iPureIntro. split; [naive_solver|].
-    rewrite right_id. by apply: prefix_app_r.
-  - simpl. iFrame "His Hbm". iFrame.
-    iExists [], _. by iFrame.
+    by rewrite right_id_L.
+  - simpl. iFrame "His Hbm". iFrame. iExists _, [] => /=.
+    rewrite spec_trace_raw_eq. by iFrame.
 Qed.
