theories/ghost_state.v
@@ -1,6 +1,6 @@
 From stdpp Require Import coPset.
 From Coq Require Import QArith Qcanon.
-From iris.algebra Require Import big_op gmap frac agree.
+From iris.algebra Require Import big_op gmap frac agree frac_agree.
 From iris.algebra Require Import csum excl auth cmra_big_op numbers.
 From iris.bi Require Import fractional.
 From iris.base_logic Require Export lib.own.
@@ -27,8 +27,8 @@ Class heapG Σ := HeapG {
   heap_backed_mem_inG :> inG Σ backed_memUR;
   heap_backed_mem_name : gname;
   heap_full_trace : list seq_label;
-  heap_spec_trace : list seq_label;
-  heap_spec_trace_inG :> ghost_varG Σ (list seq_label);
+  heap_spec_trace : list seq_label → Prop;
+  heap_spec_trace_inG :> inG Σ (frac_agreeR $ (list seq_label -d> PropO));
   heap_spec_trace_name : gname;
 }.
 
@@ -158,17 +158,25 @@ Section definitions.
   Definition mem_ctx (mem : mem_map) : iProp Σ :=
     ghost_map_auth heap_mem_name 1 mem ∗ backed_mem (dom _ mem).
 
-  Definition spec_trace_def (κs: list seq_label) : iProp Σ :=
-    ghost_var heap_spec_trace_name (1/2) κs.
+  Definition spec_trace_raw_def (Pκs: list seq_label → Prop) : iProp Σ :=
+    own heap_spec_trace_name (to_frac_agree (A:=list seq_label -d> PropO) (1/2) Pκs).
+  Definition spec_trace_raw_aux : seal (@spec_trace_raw_def). by eexists. Qed.
+  Definition spec_trace_raw := unseal spec_trace_raw_aux.
+  Definition spec_trace_raw_eq : @spec_trace_raw = @spec_trace_raw_def :=
+    seal_eq spec_trace_raw_aux.
+
+  Definition spec_trace_def (Pκs: list seq_label → Prop) : iProp Σ :=
+    ∃ Pκs' : _ → Prop, ⌜∀ x, Pκs x → Pκs' x⌝ ∗ spec_trace_raw Pκs'.
   Definition spec_trace_aux : seal (@spec_trace_def). by eexists. Qed.
   Definition spec_trace := unseal spec_trace_aux.
   Definition spec_trace_eq : @spec_trace = @spec_trace_def :=
     seal_eq spec_trace_aux.
 
   Definition spec_ctx (κs : list seq_label) : iProp Σ :=
-    ∃ κscur κsspec_end, ⌜heap_full_trace = κscur ++ κs⌝ ∗
-    ⌜heap_spec_trace = κscur ++ κsspec_end⌝ ∗
-    ghost_var heap_spec_trace_name (1/2) κsspec_end.
+    ∃ (Pκs : _ → Prop) κscur, ⌜heap_full_trace = κscur ++ κs⌝ ∗
+    ⌜heap_spec_trace κscur⌝ ∗
+    ⌜∀ κs, Pκs κs → heap_spec_trace (κscur ++ κs)⌝ ∗
+    spec_trace_raw Pκs.
 
   Definition state_ctx (σ : seq_global_state) (κs : list seq_label) : iProp Σ :=
     spec_ctx κs ∗
@@ -618,21 +626,64 @@ End mem.
 Section spec.
   Context `{!heapG Σ}.
 
-  Global Instance spec_trace_tl κs : Timeless (spec_trace κs).
+  Global Instance spec_trace_raw_tl Pκs : Timeless (spec_trace_raw Pκs).
+  Proof. rewrite spec_trace_raw_eq. by apply _. Qed.
+  Global Instance spec_trace_tl Pκs : Timeless (spec_trace Pκs).
   Proof. rewrite spec_trace_eq. by apply _. Qed.
 
-  Lemma spec_ctx_cons κ κs1 κs2:
-    spec_ctx (κ :: κs2) -∗ spec_trace (κ :: κs1) ==∗
-    spec_ctx κs2 ∗ spec_trace κs1.
+  Lemma spec_trace_raw_mono Pκs1 Pκs2 :
+    (∀ x, Pκs1 x ↔ Pκs2 x) →
+    spec_trace_raw Pκs1 -∗ spec_trace_raw Pκs2.
   Proof.
-    rewrite spec_trace_eq.
-    iDestruct 1 as (?? Hfull Hspec) "Hsc". iIntros "Hs".
-    iDestruct (ghost_var_agree with "Hsc Hs") as %?. subst.
-    iMod (ghost_var_update_halves with "Hsc Hs") as "[$ ?]".
-    iModIntro. iExists _, _. iFrame.
-    rewrite cons_middle app_assoc in Hfull.
-    rewrite cons_middle app_assoc in Hspec.
+    rewrite spec_trace_raw_eq /spec_trace_raw_def => ?.
+    by have ->: Pκs1 ≡@{_ -d> PropO} Pκs2.
+  Qed.
+
+  Lemma spec_trace_mono (Pκs1 Pκs2 : _ → Prop) :
+    (∀ x, Pκs2 x → Pκs1 x) →
+    spec_trace Pκs1 -∗ spec_trace Pκs2.
+  Proof.
+    rewrite spec_trace_eq /spec_trace_def => ?.
+    iDestruct 1 as (Pκs' ?) "Hspec". iExists _. iFrame. iPureIntro. naive_solver.
+  Qed.
+
+  Lemma spec_trace_raw_agree Pκs1 Pκs2 :
+    spec_trace_raw Pκs1 -∗ spec_trace_raw Pκs2 -∗ ⌜∀ x, Pκs1 x ↔ Pκs2 x⌝.
+  Proof.
+    rewrite spec_trace_raw_eq. iIntros "Ht1 Ht2".
+    iDestruct (own_valid_2 with "Ht1 Ht2") as %[Hq Ha]%frac_agree_op_valid.
     done.
+  Qed.
+
+  Lemma spec_trace_raw_update Pκs1 Pκs2 Pκs :
+    spec_trace_raw Pκs1 -∗ spec_trace_raw Pκs2 ==∗ spec_trace_raw Pκs ∗ spec_trace_raw Pκs.
+  Proof.
+    iIntros "H1 H2".
+    iDestruct (spec_trace_raw_agree with "H1 H2") as %Heq.
+    iDestruct (spec_trace_raw_mono with "H1") as "H1"; [done|].
+    rewrite spec_trace_raw_eq /spec_trace_raw_def.
+    iCombine "H1 H2" as "H". rewrite -frac_agree_op Qp_half_half.
+    iMod (own_update _ _ (to_frac_agree (A:= _ -d> _) 1 Pκs) with "H") as "H".
+    { by apply cmra_update_exclusive. }
+    rewrite -{1}Qp_half_half frac_agree_op own_op.
+    by iFrame.
+  Qed.
+
+  Lemma spec_ctx_cons κ κs (Pκs : _ → Prop):
+    Pκs [κ] →
+    spec_ctx (κ :: κs) -∗ spec_trace Pκs ==∗
+    spec_ctx κs ∗ spec_trace (λ κs, Pκs (κ::κs)).
+  Proof.
+    move => Hκ.
+    iDestruct 1 as (HPκs'' κscur Hfull Hspec ?) "Hsc".
+    rewrite spec_trace_eq. iDestruct 1 as (Pκs' HPκs') "Hs".
+    iDestruct (spec_trace_raw_agree with "Hsc Hs") as %HPκs.
+    iMod (spec_trace_raw_update with "Hsc Hs") as "[Ht ?]".
+    iModIntro. iSplitR "Ht". 2: { iExists (λ κs, Pκs (κ :: κs)). by iFrame. }
+    iExists _, (κscur ++ [κ]). iFrame. iPureIntro. split_and!.
+    - by rewrite -app_assoc -cons_middle.
+    - naive_solver.
+    - move => ?. rewrite -app_assoc -cons_middle. naive_solver.
   Qed.
 
 End spec.
